curve25519-dalek/translated/TypesExternal.lean
@@ -1,4 +1,12 @@
+/-
+Copyright (c) 2026 The Beneficial AI Foundation. All rights reserved.
+Released under Apache 2.0 license as described in the file LICENSE.
+Authors: Wojciech Aleksander Wołoszyn
+-/
 import Aeneas
+
+/-! External type models. -/
+
 open Aeneas Aeneas.Std Result ControlFlow Error
 set_option linter.dupNamespace false
 set_option linter.hashCommand false
@@ -18,4 +26,6 @@ set_option maxRecDepth 2048
     Name pattern: [subtle::Choice]
     Visibility: public -/
 @[rust_type "subtle::Choice"]
-axiom subtle.Choice : Type
+structure subtle.Choice where
+  /-- The unrestricted raw byte. -/
+  val : U8
