Dalek32/Subtle/ChoiceFromU8.lean
@@ -1,0 +1,29 @@
+/-
+Copyright (c) 2026 The Beneficial AI Foundation. All rights reserved.
+Released under Apache 2.0 license as described in the file LICENSE.
+Authors: Wojciech Aleksander Wołoszyn
+-/
+import Dalek32.Lint.Basic
+import translated.FunsExternal
+
+/-!
+# `Choice::from`
+
+Preserves input bytes 0 and 1.
+Source: "subtle-2.6.1/src/lib.rs", lines 238-244.
+-/
+
+open Aeneas Aeneas.Std Result Aeneas.Std.WP
+
+namespace subtle.Choice.Insts.CoreConvertFromU8
+
+/-- **Spec theorem for `<subtle::Choice as core::convert::From<u8>>::from`**
+
+Preserves 0 or 1. -/
+@[step]
+theorem from_spec (input : U8) (h_input : input = 0#u8 ∨ input = 1#u8) :
+    «from» input ⦃ (choice : subtle.Choice) =>
+      choice.val = input ⦄ := by
+  simp [«from», h_input]
+
+end subtle.Choice.Insts.CoreConvertFromU8
